src/tls/QUIC.fst
@@ -24,6 +24,8 @@ open FFICallbacks
 
 module HS = FStar.HyperStack
 module FFI = FFI
+module Range = Range
+open Range
 
 #set-options "--admit_smt_queries true"
 
@@ -195,34 +197,162 @@ type chSummary = {
   ch_cookie: option bytes;
 }
 
-let peekClientHello (ch:bytes) : ML (option chSummary) =
+let peekClientHello (ch:bytes) (has_record:bool) : ML (option chSummary) =
   if length ch < 40 then (trace "peekClientHello: too short"; None) else
-  let hdr, ch = split ch 5ul in
-  match Record.parseHeader hdr with
-  | Error (_, msg) -> trace ("peekClientHello: bad record header"); None
-  | Correct(ct, pv, len) ->
-    if ct <> Content.Handshake || len <> length ch then
-      (trace "peekClientHello: bad CT or length"; None)
-    else
-      match HandshakeMessages.parseMessage ch with
-      | Error _
-      | Correct None -> trace ("peekClientHello: bad handshake header"); None
-      | Correct (Some (| _, hst, ch, _ |)) ->
-        if hst <> HandshakeMessages.HT_client_hello then
-          (trace "peekClientHello: not a client hello"; None)
-        else
-          match HandshakeMessages.parseClientHello ch with
-          | Error (_, msg) -> trace ("peekClientHello: bad client hello: "^msg); None
-          | Correct (ch, _) ->
-            let sni = Negotiation.get_sni ch in
-            let alpn = Extensions.alpnBytes (Negotiation.get_alpn ch) in
-            let ext = HandshakeMessages.optionExtensionsBytes ch.HandshakeMessages.ch_extensions in
-            let cookie =
-              match Negotiation.find_cookie ch with
+  let ch =
+    if has_record then
+      let hdr, ch = split ch 5ul in
+      match Record.parseHeader hdr with
+      | Error (_, msg) -> trace ("peekClientHello: bad record header"); None
+      | Correct(ct, pv, len) ->
+        if ct <> Content.Handshake || len <> length ch then
+          (trace "peekClientHello: bad CT or length"; None)
+        else Some ch
+    else Some ch
+    in
+  match ch with
+  | None -> None
+  | Some ch ->
+    match HandshakeMessages.parseMessage ch with
+    | Error _
+    | Correct None -> trace ("peekClientHello: bad handshake header"); None
+    | Correct (Some (| _, hst, ch, _ |)) ->
+      if hst <> HandshakeMessages.HT_client_hello then
+         (trace "peekClientHello: not a client hello"; None)
+      else
+        match HandshakeMessages.parseClientHello ch with
+        | Error (_, msg) -> trace ("peekClientHello: bad client hello: "^msg); None
+        | Correct (ch, _) ->
+          let sni = Negotiation.get_sni ch in
+          let alpn = Extensions.alpnBytes (Negotiation.get_alpn ch) in
+          let ext = HandshakeMessages.optionExtensionsBytes ch.HandshakeMessages.ch_extensions in
+          let cookie =
+            match Negotiation.find_cookie ch with
+            | None -> None
+            | Some c ->
+              match Ticket.check_cookie c with
               | None -> None
-              | Some c ->
-                match Ticket.check_cookie c with
-                | None -> None
-                | Some (hrr, digest, extra) -> Some extra
-              in
-            Some ({ch_sni = sni; ch_alpn = alpn; ch_extensions = ext; ch_cookie = cookie; })
+              | Some (hrr, digest, extra) -> Some extra
+            in
+          Some ({ch_sni = sni; ch_alpn = alpn; ch_extensions = ext; ch_cookie = cookie; })
+
+// QUIC interface to TLS handshake
+
+module H = Old.Handshake
+module HSL = HandshakeLog
+
+let create_hs (is_server:bool) config : ML H.hs =
+  let r = new_region HS.root in
+  let role = if is_server then Server else Client in
+  H.create r config role
+
+type hs_in = {
+  input: bytes;
+  max_output: UInt32.t;
+}
+
+type hs_out = {
+  consumed: UInt32.t;
+  output: bytes;
+  to_be_written: UInt32.t;
+  is_complete: bool;
+}
+
+type hs_result =
+  | HS_SUCCESS of hs_out
+  | HS_ERROR of UInt16.t
+
+private let currentId (hs:H.hs) (rw:rw) : St TLSInfo.id =
+  let j = H.i hs rw in
+  if j<0 then PlaintextID (H.nonce hs)
+  else
+    let e = Old.Epochs.get_current_epoch (H.epochs_of hs) rw in
+    Old.Epochs.epoch_id e
+
+let get_epochs (hs:H.hs) : ML (int * int) =
+  H.i hs Reader, H.i hs Writer
+
+private let handle_signals (hs:H.hs) (sig:option HSL.next_keys_use) : ML unit =
+  match sig with
+  | None -> ()
+  | Some use ->
+    Old.Epochs.incr_writer (H.epochs_of hs);
+    if use.HSL.out_skip_0RTT then
+      Old.Epochs.incr_writer (H.epochs_of hs)
+
+let process_hs (hs:H.hs) (ctx:hs_in) : ML hs_result =
+  let tbw = H.to_be_written hs in
+  if tbw > 0 then
+   begin
+    if ctx.max_output = 0ul then
+      HS_SUCCESS ({
+        consumed = 0ul;
+        output = empty_bytes;
+	to_be_written = UInt32.uint_to_t tbw;
+	is_complete = false;
+      })
+    else
+      let i = currentId hs Writer in
+      match H.next_fragment_bounded hs i (UInt32.v ctx.max_output) with
+      | Error (z) -> HS_ERROR 1us
+      | Correct (HSL.Outgoing (Some frag) sig _) ->
+        handle_signals hs sig;
+        HS_SUCCESS ({
+	  consumed = 0ul;
+	  output = dsnd frag;
+	  to_be_written = UInt32.uint_to_t (H.to_be_written hs);
+	  is_complete = false;
+	})
+   end
+  else
+    let i = currentId hs Reader in
+    let len = length ctx.input in
+    let rg : Range.frange i = (len, len) in
+    let f : Range.rbytes rg = ctx.input in
+    match H.recv_fragment hs rg f with
+    | H.InQuery _ _ -> HS_ERROR 2us
+    | H.InError z -> HS_ERROR 3us
+    | H.InAck nk complete ->
+      let consumed = UInt32.uint_to_t len in
+      let i = currentId hs Writer in
+      match H.next_fragment_bounded hs i (UInt32.v ctx.max_output) with
+      | Error z -> HS_ERROR 4us
+      | Correct (HSL.Outgoing frag sig _ ) ->
+        handle_signals hs sig;
+	HS_SUCCESS ({
+          consumed = consumed;
+          output = (match frag with Some f -> dsnd f | None -> empty_bytes);
+          to_be_written = UInt32.uint_to_t (H.to_be_written hs);
+          is_complete = complete;
+        })
+
+type raw_key = {
+  alg: aeadAlg;
+  aead_key: bytes;
+  aead_iv: bytes;
+  pn_key: bytes;
+}
+
+let get_key (hs:Old.Handshake.hs) (ectr:nat) (rw:bool) : ML (option raw_key) =
+  let epochs = Monotonic.Seq.i_read (Old.Epochs.get_epochs (Handshake.epochs_of hs)) in
+  if Seq.length epochs <= ectr then None
+  else
+    let AEAD alg _ = aeAlg_of_id (currentId hs Writer) in
+    let e = Seq.index epochs ectr in
+    let key, iv =
+      if rw then
+        let StAE.Stream _ st = Old.Epochs.reader_epoch e in
+        let st = StreamAE.State?.aead st in
+        AEADProvider.leak st
+      else
+        let StAE.Stream _ st = Old.Epochs.writer_epoch e in
+        let st = StreamAE.State?.aead st in
+        AEADProvider.leak st
+    in
+    Some ({
+      alg = alg;
+      aead_key = key;
+      aead_iv = iv;
+      pn_key = Bytes.create 32ul 0uy
+    })
+    
